fv: add double gadget

fv/lean/Ragu/Circuits/Point/Spec.lean
@@ -1,7 +1,8 @@
 import Clean.Circuit
-import Clean.Utils.Primes
+import Ragu.Core
 
 namespace Ragu.Circuits.Point.Spec
+open Core.Primes
 variable {p : ℕ} [Fact p.Prime]
 
 structure Point (F : Type) where
@@ -9,9 +10,12 @@ structure Point (F : Type) where
   y : F
 deriving ProvableStruct
 
+
+
 /--
-  NOTE: supports only short Weirstrass curves with a = 0
-  TODO: replace with Weirstrass in Mathlib
+  NOTE: supports only short Weierstrass curves with a = 0
+
+  TODO: replace with Weierstrass in Mathlib
 -/
 structure CurveParams (F : Type) where
   b : F
@@ -19,7 +23,11 @@ structure CurveParams (F : Type) where
 def Point.isOnCurve (point : Point (F p)) (curveParams : CurveParams (F p)) : Prop :=
   point.y^2 = point.x^3 + curveParams.b
 
+def CurveParams.noOrderTwoPoints (curveParams : CurveParams (F p)) : Prop :=
+  (∀ point : Spec.Point (F p), (point.isOnCurve curveParams) → point.y ≠ 0)
+
 def Point.double (point : Point (F p)) : Point (F p) :=
+  -- TODO: a / 0 is defined to be 0 for fields, this is not a precise spec
   let lambda := (3 * point.x^2) / (2 * point.y)
   let x2 := lambda^2 - 2*point.x
   {
@@ -27,4 +35,29 @@ def Point.double (point : Point (F p)) : Point (F p) :=
     y := lambda * (point.x - x2) - point.y
   }
 
+-- concrete pasta curves parameters
+def EpAffineParams: Circuits.Point.Spec.CurveParams Core.Primes.Fp := {b := 5}
+def EqAffineParams: Circuits.Point.Spec.CurveParams Core.Primes.Fq := {b := 5}
+
 end Ragu.Circuits.Point.Spec
+
+namespace Ragu.Circuits.Point.Lemmas
+variable {p : ℕ} [Fact p.Prime] [NeZero (2 : F p)]
+open Spec
+
+lemma double_preserves_membership (point : Point (F p)) (curveParams: CurveParams (F p))
+    (h_membership: point.isOnCurve curveParams) (h_order : curveParams.noOrderTwoPoints) :
+    point.double.isOnCurve curveParams := by
+  simp only [CurveParams.noOrderTwoPoints] at h_order
+  specialize h_order point h_membership
+  simp only [Point.isOnCurve, Point.double]
+  simp only [Point.isOnCurve] at h_membership
+  have h2 : (2 : F p) ≠ 0 := NeZero.ne 2
+  have h2y : (2 : F p) * point.y ≠ 0 := mul_ne_zero h2 h_order
+  field_simp [h_order, h2y, h2]
+  have hb : curveParams.b = point.y ^ 2 - point.x ^ 3 := by rw [h_membership]; ring
+  rw [hb]
+  ring
+
+
+end Ragu.Circuits.Point.Lemmas
