fv/lean/Ragu/Circuits/Point/Double.lean
@@ -1,0 +1,93 @@
+import Clean.Circuit
+import Clean.Utils.Primes
+import Ragu.Circuits.Element.AllocSquare
+import Ragu.Circuits.Element.Mul
+import Ragu.Circuits.Element.Square
+import Ragu.Circuits.Element.DivNonzero
+import Ragu.Circuits.Point.Spec
+
+namespace Ragu.Circuits.Point.Double
+variable {p : ℕ} [Fact p.Prime] [NeZero (2 : F p)]
+
+def main (input : Var Spec.Point (F p)) : Circuit (F p) (Var Spec.Point (F p)) := do
+  let ⟨x, y⟩ := input
+
+  -- delta = 3x^2 / 2y
+  let double_y := y + y
+  let ⟨x2⟩ ← subcircuit Element.Square.circuit ⟨x⟩
+  let x2_scaled := (3 : F p) * x2
+  let delta ← subcircuit Element.DivNonzero.circuit ⟨x2_scaled, double_y⟩
+
+  -- x3 = delta^2 - 2x
+  let double_x := x + x
+  let ⟨delta2⟩ ← subcircuit Element.Square.circuit ⟨delta⟩
+  let x3 := delta2 - double_x
+
+  -- y3 = delta * (x - x3) - y
+  let x_sub_x3 := x - x3
+  let delta_x_sub_3 ← subcircuit Element.Mul.circuit ⟨delta, x_sub_x3⟩
+  let y3 := delta_x_sub_3 - y
+
+  return ⟨x3, y3⟩
+
+def Assumptions (curveParams : Spec.CurveParams (F p)) (input : Spec.Point (F p)) :=
+  input.isOnCurve curveParams ∧
+  -- for the circuit to be sound, there must not exist points of order 2 on the curve,
+  -- therefore soundness is also conditioned on the following property:
+  curveParams.noOrderTwoPoints
+
+def Spec (curveParams : Spec.CurveParams (F p)) (input : Spec.Point (F p)) (output : Spec.Point (F p)) :=
+  output = input.double ∧
+  output.isOnCurve curveParams
+
+instance elaborated : ElaboratedCircuit (F p) Spec.Point Spec.Point where
+  main
+  localLength _ := 12
+
+theorem soundness (curveParams : Spec.CurveParams (F p)) : Soundness (F p) elaborated (Assumptions curveParams) (Spec curveParams) := by
+  circuit_proof_start
+  simp [circuit_norm,
+    Element.Square.circuit, Element.Square.Assumptions, Element.Square.Spec,
+    Element.DivNonzero.circuit, Element.DivNonzero.Assumptions, Element.DivNonzero.Spec,
+    Element.Mul.circuit, Element.Mul.Assumptions, Element.Mul.Spec
+  ] at h_holds ⊢
+
+  obtain ⟨c1, c2, c3, c4⟩ := h_holds
+
+  obtain ⟨h_membership, h_order⟩ := h_assumptions
+  have h : input_y + input_y ≠ 0 := by
+    have hy : input_y ≠ 0 := h_order ⟨input_x, input_y⟩ h_membership
+    rw [← two_mul]
+    exact mul_ne_zero (NeZero.ne 2) hy
+
+  simp [h, c1] at c2
+  rw [c2] at c3 c4
+  rw [c3] at c4
+  clear c1 c2
+
+  simp [Spec.Point.double]
+
+  constructor
+  · rw [c3, c4]
+    ring_nf
+    simp only [and_self]
+  · rw [c3, c4]
+    have h := Lemmas.double_preserves_membership ⟨input_x, input_y⟩ curveParams h_membership h_order
+    simp [Spec.Point.double] at h
+    ring_nf at ⊢ h
+    exact h
+
+
+theorem completeness (curveParams : Spec.CurveParams (F p)) : Completeness (F p) elaborated (Assumptions curveParams) := by
+  sorry
+
+def circuit (curveParams : Spec.CurveParams (F p)) : FormalCircuit (F p) Spec.Point Spec.Point :=
+  {
+    elaborated with
+    Assumptions := Assumptions curveParams,
+    Spec := Spec curveParams,
+    soundness := soundness curveParams,
+    completeness := completeness curveParams
+  }
+
+end Ragu.Circuits.Point.Double
